ulib/FStar.Monotonic.Seq.fst
@@ -47,7 +47,7 @@ abstract let grows (#a:Type) (s1:seq a) (s3:seq a) =
   
 let seq_extension_reflexive (#a:Type) (s:seq a) 
   : Lemma (ensures (grows s s)) 
-  = exists_intro (fun w -> seq_extension s w s) (Seq.createEmpty #a)
+  = exists_intro (fun w -> seq_extension s w s) (Seq.empty #a)
 
 let seq_extension_transitive (s1:seq 'a) (s2:seq 'a) (s3:seq 'a) (s1':seq 'a) (s2':seq 'a) 
   : Lemma ((seq_extension s1 s1' s2 /\ seq_extension s2 s2' s3)
@@ -220,7 +220,7 @@ let un_snoc #a s =
 val map: ('a -> Tot 'b) -> s:seq 'a -> Tot (seq 'b)
     (decreases (Seq.length s))
 let rec map f s =
-  if Seq.length s = 0 then Seq.createEmpty
+  if Seq.length s = 0 then Seq.empty
   else let prefix, last = un_snoc s in
        SeqP.snoc (map f prefix) (f last)
 
@@ -321,7 +321,7 @@ let map_has_at_index_stable (#a:Type) (#b:Type) (#i:rid)
 val collect: ('a -> Tot (seq 'b)) -> s:seq 'a -> Tot (seq 'b)
     (decreases (Seq.length s))
 let rec collect f s =
-  if Seq.length s = 0 then Seq.createEmpty
+  if Seq.length s = 0 then Seq.empty
   else let prefix, last = un_snoc s in
        Seq.append (collect f prefix) (f last)
 
